WIP

src/Parsers/DependentlyTypedOption.v
@@ -58,9 +58,11 @@ Section recursive_descent_parser.
   Local Instance option_methods : @parser_computational_dataT _ String
     := { methods' := option_methods' }.
 
-  Context (strdata : @parser_computational_strdataT _ String G {| DependentlyTyped.methods' := methods' |}).
+  Local Notation orig_methods := {| DependentlyTyped.methods' := methods' |}.
 
-  Local Instance option_strdata : @parser_computational_strdataT _ String G option_methods
+  Context (strdata : @parser_computational_strdataT _ String G orig_methods).
+
+  Global Instance option_strdata : @parser_computational_strdataT _ String G option_methods
     := { lower_nonterminal_name_state str0 valid nonterminal_name s
          := option_map (@lower_nonterminal_name_state _ _ _ _ strdata _ _ _ _);
          lower_string_head str0 valid prod prods s
@@ -71,4 +73,212 @@ Section recursive_descent_parser.
          := option_map (@lift_lookup_nonterminal_name_state_lt _ _ _ _ strdata _ _ _ _ pf);
          lift_lookup_nonterminal_name_state_eq str0 valid nonterminal_name s pf
          := option_map (@lift_lookup_nonterminal_name_state_eq _ _ _ _ strdata _ _ _ _ pf) }.
+
+  Context (types_success_data' : @parser_dependent_types_success_dataT' _ String orig_methods).
+
+  Definition option_rect_str {A} {B : StringWithSplitState String (fun s => option (A s)) -> Type}
+             (f : forall x : StringWithSplitState String A, B (lift_StringWithSplitState x (@Some _)))
+             (none_case : forall s, B {| string_val := s; state_val := None |})
+             (x : StringWithSplitState String (fun s => option (A s)))
+  : B x
+    := match x return B x with
+         | {| string_val := s ; state_val := None |} => none_case s
+         | {| string_val := s ; state_val := Some st |}
+           => f {| string_val := s ; state_val := st |}
+       end.
+
+  Global Instance option_stypes' : @parser_dependent_types_success_dataT' _ String option_methods
+    := { T_nonterminal_name_success str0 valid name
+         := option_rect_str (@T_nonterminal_name_success _ _ _ types_success_data' str0 valid name) (fun _ => True);
+         T_item_success str0 valid it
+         := option_rect_str (@T_item_success _ _ _ types_success_data' str0 valid it) (fun _ => True);
+         T_production_success str0 valid prod
+         := option_rect_str (@T_production_success _ _ _ types_success_data' str0 valid prod) (fun _ => True) ;
+         T_productions_success str0 valid prods
+         := option_rect_str (@T_productions_success _ _ _ types_success_data' str0 valid prods) (fun _ => True)  }.
+
+  Definition option_types_success_data : @parser_dependent_types_success_dataT _ String :=
+    {| methods := option_methods;
+       stypes' := option_stypes' |}.
+
+  Global Instance option_types_failure_data' : @parser_dependent_types_failure_dataT' _ String option_methods
+    := { T_nonterminal_name_failure str0 valid name
+         := option_rect_str (@T_nonterminal_name_failure _ _ _ types_failure_data' str0 valid name) (fun _ => True);
+         T_item_failure str0 valid it
+         := option_rect_str (@T_item_failure _ _ _ types_failure_data' str0 valid it) (fun _ => True);
+         T_production_failure str0 valid prod
+         := option_rect_str (@T_production_failure _ _ _ types_failure_data' str0 valid prod) (fun _ => True) ;
+         T_productions_failure str0 valid prods
+         := option_rect_str (@T_productions_failure _ _ _ types_failure_data' str0 valid prods) (fun _ => True)  }.
+          : forall (str0 : String) (valid : nonterminal_names_listT)
+                   (name : string)
+                   (str : StringWithSplitState String (split_stateT str0 valid (include_nonterminal_name _ name))),
+              Type;
+          T_item_failure
+          : forall (str0 : String) (valid : nonterminal_names_listT)
+                   (it : item CharType)
+                   (str : StringWithSplitState String (split_stateT str0 valid it)),
+              Type;
+          T_production_success
+          : forall (str0 : String) (valid : nonterminal_names_listT)
+                   (prod : production CharType)
+                   (str : StringWithSplitState String (split_stateT str0 valid prod)),
+              Type;
+
+          T_productions_success
+          : forall (str0 : String) (valid : nonterminal_names_listT)
+                   (prods : productions CharType)
+                   (str : StringWithSplitState String (split_stateT str0 valid prods)),
+              Type }.
+
+      Class parser_dependent_types_success_dataT :=
+        { methods :> parser_computational_dataT;
+          stypes' :> parser_dependent_types_success_dataT' }.
+
+      Class parser_dependent_types_failure_dataT' `{parser_dependent_types_success_dataT} :=
+        { T_nonterminal_name_failure
+          : forall (str0 : String) (valid : nonterminal_names_listT)
+                   (name : string)
+                   (str : StringWithSplitState String (split_stateT str0 valid (include_nonterminal_name _ name))),
+              Type;
+          T_item_failure
+          : forall (str0 : String) (valid : nonterminal_names_listT)
+                   (it : item CharType)
+                   (str : StringWithSplitState String (split_stateT str0 valid it)),
+              Type;
+          T_production_failure
+          : forall (str0 : String) (valid : nonterminal_names_listT)
+                   (prod : production CharType)
+                   (str : StringWithSplitState String (split_stateT str0 valid prod)),
+              Type;
+
+          split_string_lift_T
+            (str0 : String) (valid : nonterminal_names_listT)
+            (it : item CharType) (its : production CharType)
+            (str : StringWithSplitState String (split_stateT str0 valid (it::its : production CharType)))
+            (split : list
+                       (StringWithSplitState String (split_stateT str0 valid it) *
+                        StringWithSplitState String (split_stateT str0 valid its)))
+          := str ≤s str0
+             -> fold_right
+                  Datatypes.prod
+                  unit
+                  (map (fun s1s2 =>
+                          let s1 := fst s1s2 in
+                          let s2 := snd s1s2 in
+                          ((T_item_failure str0 valid it s1 * T_production_failure str0 valid its s2)
+                           + (T_item_success str0 valid it s1 * T_production_failure str0 valid its s2)
+                           + (T_item_failure str0 valid it s1 * T_production_success str0 valid its s2))%type)
+                       split)
+             -> T_production_failure str0 valid (it::its) str;
+
+          T_productions_failure
+          : forall (str0 : String) (valid : nonterminal_names_listT)
+                   (prods : productions CharType)
+                   (str : StringWithSplitState String (split_stateT str0 valid prods)),
+              Type }.
+
+      Class parser_dependent_types_dataT :=
+        { stypes :> parser_dependent_types_success_dataT;
+          ftypes' :> parser_dependent_types_failure_dataT' }.
+
+      Class parser_dependent_types_extra_success_dataT' `{types : parser_dependent_types_success_dataT, @parser_computational_strdataT (@methods types)} :=
+        { lift_success
+          : forall {str0 valid} nonterminal_name {str},
+              @T_nonterminal_name_success _ _ str0 valid nonterminal_name (lift_StringWithSplitState str lower_nonterminal_name_state)
+              -> @T_item_success _ _ str0 valid (NonTerminal _ nonterminal_name) str;
+          parse_terminal_success
+          : forall {str0 valid} ch {str},
+              let ret := @T_item_success _ _ str0 valid (Terminal ch) str in
+              [[ ch ]] =s str -> ret;
+          parse_empty_success
+          : forall {str0 valid str},
+              let ret := @T_production_success _ _ str0 valid nil str in
+              str =s Empty _ -> ret;
+          cons_success
+          : forall {str0 valid} it its {s1 s2 str},
+              let a1 := @T_item_success _ _ str0 valid it s1 in
+              let a2 := @T_production_success _ _ str0 valid its s2 in
+              let ret := @T_production_success _ _ str0 valid (it::its) str in
+              str ≤s str0 -> s1 ++ s2 =s str -> In (s1, s2) (split_string_for_production str0 valid it its str) -> a1 -> a2 -> ret;
+
+          lift_prods_success_head
+          : forall {str0 valid prod prods str},
+              let ret := @T_productions_success _ _ str0 valid (prod::prods) str in
+              let arg := @T_production_success _ _ str0 valid prod (lift_StringWithSplitState str lower_string_head) in
+              arg -> ret;
+          lift_prods_success_tail
+          : forall {str0 valid prod prods str},
+              let ret := @T_productions_success _ _ str0 valid (prod::prods) str in
+              let arg := @T_productions_success _ _ str0 valid prods (lift_StringWithSplitState str lower_string_tail) in
+              arg -> ret;
+
+          lift_parse_nonterminal_name_success_lt
+          : forall {str0 valid nonterminal_name str},
+              let ret := @T_nonterminal_name_success _ _ str0 valid nonterminal_name str in
+              forall (pf : Length str < Length str0),
+                let arg := @T_productions_success _ _ str initial_nonterminal_names_data (Lookup G nonterminal_name) (lift_StringWithSplitState str (lift_lookup_nonterminal_name_state_lt pf)) in
+                arg -> ret;
+          lift_parse_nonterminal_name_success_eq
+          : forall {str0 valid nonterminal_name str},
+              let ret := @T_nonterminal_name_success _ _ str0 valid nonterminal_name str in
+              forall (pf : str = str0 :> String),
+                let arg := @T_productions_success _ _ str0 (remove_nonterminal_name valid nonterminal_name) (Lookup G nonterminal_name) (lift_StringWithSplitState str (lift_lookup_nonterminal_name_state_eq pf)) in
+
+                is_valid_nonterminal_name valid nonterminal_name = true -> arg -> ret
+        }.
+
+      Class parser_dependent_types_extra_failure_dataT' `{types : parser_dependent_types_dataT, @parser_computational_strdataT (@methods (@stypes types))} :=
+        { lift_failure
+          : forall {str0 valid} nonterminal_name {str},
+              @T_nonterminal_name_failure _ _ str0 valid nonterminal_name (lift_StringWithSplitState str lower_nonterminal_name_state)
+              -> @T_item_failure _ _ str0 valid (NonTerminal _ nonterminal_name) str;
+          parse_terminal_failure
+          : forall {str0 valid} ch {str},
+              let ret := @T_item_failure _ _ str0 valid (Terminal ch) str in
+              ([[ ch ]] =s str) = false -> ret;
+          parse_empty_failure
+          : forall {str0 valid str},
+              let ret := @T_production_failure _ _ str0 valid nil str in
+              str ≤s str0 -> (str =s Empty _) = false -> ret;
+
+          fail_parse_nil_productions
+          : forall {str0 valid str}, T_productions_failure str0 valid [] str;
+          lift_prods_failure
+          : forall {str0 valid prod prods str},
+              let ret := @T_productions_failure _ _ str0 valid (prod::prods) str in
+              let a1 := @T_production_failure _ _ str0 valid prod (lift_StringWithSplitState str lower_string_head) in
+              let a2 := @T_productions_failure _ _ str0 valid prods (lift_StringWithSplitState str lower_string_tail) in
+              a1 -> a2 -> ret;
+
+          H_prod_split : forall str0 valid it its str, split_string_lift_T str0 valid it its str (split_string_for_production str0 valid it its str);
+
+
+          lift_parse_nonterminal_name_failure_lt
+          : forall {str0 valid nonterminal_name str},
+              let ret := @T_nonterminal_name_failure _ _ str0 valid nonterminal_name str in
+              forall (pf : Length str < Length str0),
+                let arg := @T_productions_failure _ _ str initial_nonterminal_names_data (Lookup G nonterminal_name) (lift_StringWithSplitState str (lift_lookup_nonterminal_name_state_lt pf)) in
+                arg -> ret;
+          lift_parse_nonterminal_name_failure_eq
+          : forall {str0 valid nonterminal_name str},
+              let ret := @T_nonterminal_name_failure _ _ str0 valid nonterminal_name str in
+              forall (pf : str = str0 :> String),
+                let arg := @T_productions_failure _ _ str0 (remove_nonterminal_name valid nonterminal_name) (Lookup G nonterminal_name) (lift_StringWithSplitState str (lift_lookup_nonterminal_name_state_eq pf)) in
+                arg -> ret;
+
+          elim_parse_nonterminal_name_failure
+          : forall {str0 valid nonterminal_name str},
+              let ret := @T_nonterminal_name_failure _ _ str0 valid nonterminal_name str in
+              str ≤s str0
+              -> ~ Length str < Length str0
+              -> is_valid_nonterminal_name valid nonterminal_name = false
+              -> ret
+        }.
+
+      Class parser_dependent_types_extra_dataT :=
+        { types :> parser_dependent_types_dataT;
+          strdata :> parser_computational_strdataT;
+          extra_success_data :> parser_dependent_types_extra_success_dataT';
+          extra_failure_data :> parser_dependent_types_extra_failure_dataT' }.
 End recursive_descent_parser.
